theories/Gen/Bidirectional.v
@@ -39,10 +39,12 @@ Set Implicit Arguments.
 Section Generator.
   Import MonadNotations.
 
-  Fixpoint check
-    `{lkReflΘ: LkRefl Θ, lkTransΘ: LkTrans Θ, lkStepΘ: LkStep Θ} {reflTransΘ: ReflTrans Θ}
-    `{pureM:Pure M, bindM:Bind Θ M, failM:Fail M, tcM:TypeCheckM M}
-    (e : Exp) : ⊧ OEnv ⇢ OTy ⇢ M OExp :=
+  (* We would normally like to introduce the typeclass instances using Context,
+     but for some reason that causes the fixpoint to stay unfolded in the
+     proofs. *)
+  Fixpoint ocheck `{lkReflΘ: LkRefl Θ, lkTransΘ: LkTrans Θ, lkStepΘ: LkStep Θ,
+    reflTransΘ: !ReflTrans Θ, pureM:Pure M, bindM:Bind Θ M, failM:Fail M,
+    tcM:TypeCheckM M} (e : Exp) : ⊧ OEnv ⇢ OTy ⇢ M OExp :=
     fun w Γ τ =>
       match e with
       | exp.var x =>
@@ -58,29 +60,29 @@ Section Generator.
           _ <- equals τ oty.bool ;;
           pure oexp.false
       | exp.ifte e1 e2 e3 =>
-          e1' <- check e1 Γ oty.bool ;;
-          e2' <- check e2 Γ[_] τ[_] ;;
-          e3' <- check e3 Γ[_] τ[_] ;;
+          e1' <- ocheck e1 Γ oty.bool ;;
+          e2' <- ocheck e2 Γ[_] τ[_] ;;
+          e3' <- ocheck e3 Γ[_] τ[_] ;;
           pure (oexp.ifte e1'[_] e2'[_] e3')
       | exp.absu x e =>
           t1  <- pick ;;
           t2  <- pick ;;
           _   <- equals τ[_] (oty.func t1[_] t2) ;;
-          e'  <- check e (Γ[_] ,, x∷t1[_]) t2[_] ;;
+          e'  <- ocheck e (Γ[_] ,, x∷t1[_]) t2[_] ;;
           pure (oexp.abst x t1[_] e')
       | exp.abst x t1 e =>
           τ2  <- pick ;;
           _   <- equals τ[_] (oty.func (lift t1) τ2) ;;
-          e'  <- check e (Γ[_] ,, x∷lift t1) τ2[_] ;;
+          e'  <- ocheck e (Γ[_] ,, x∷lift t1) τ2[_] ;;
           pure (oexp.abst x (lift t1) e')
       | exp.app e1 e2 =>
-         '(τ2,e2') <- synth e2 Γ ;;
-         e1'       <- check e1 Γ[_] (oty.func τ2 τ[_]) ;;
+         '(τ2,e2') <- osynth e2 Γ ;;
+         e1'       <- ocheck e1 Γ[_] (oty.func τ2 τ[_]) ;;
          pure (oexp.app e1' e2'[_])
       end
-  with synth `{lkReflΘ: LkRefl Θ, lkTransΘ: LkTrans Θ, lkStepΘ: LkStep Θ} {reflTransΘ: ReflTrans Θ}
-         `{pureM:Pure M, bindM:Bind Θ M, failM:Fail M, tcM:TypeCheckM M}
-  (e : Exp) : ⊧ OEnv ⇢ M (OTy * OExp) :=
+  with osynth `{lkReflΘ: LkRefl Θ, lkTransΘ: LkTrans Θ, lkStepΘ: LkStep Θ,
+    reflTransΘ: !ReflTrans Θ, pureM:Pure M, bindM:Bind Θ M, failM:Fail M,
+    tcM:TypeCheckM M} (e : Exp) : ⊧ OEnv ⇢ M (OTy * OExp) :=
     fun w Γ =>
       match e with
       | exp.var x =>
@@ -91,23 +93,23 @@ Section Generator.
       | exp.true  => pure (oty.bool, oexp.true)
       | exp.false => pure (oty.bool, oexp.false)
       | exp.ifte e1 e2 e3 =>
-          e1'        <- check e1 Γ oty.bool ;;
-          '(τ,e2')   <- synth e2 Γ[_] ;;
-          e3'        <- check e3 Γ[_] τ ;;
+          e1'        <- ocheck e1 Γ oty.bool ;;
+          '(τ,e2')   <- osynth e2 Γ[_] ;;
+          e3'        <- ocheck e3 Γ[_] τ ;;
           pure (τ[_], oexp.ifte e1'[_] e2'[_] e3')
       | exp.absu x e =>
           t1         <- pick ;;
-          '(t2,e')   <- synth e (insert (M := OEnv _) x t1 Γ[_]) ;;
+          '(t2,e')   <- osynth e (insert (M := OEnv _) x t1 Γ[_]) ;;
           pure (oty.func t1[_] t2, oexp.abst x t1[_] e')
       | exp.abst x t1 e =>
-          '(t2,e')   <- synth e (insert (M := OEnv _) x (lift t1) Γ) ;;
+          '(t2,e')   <- osynth e (insert (M := OEnv _) x (lift t1) Γ) ;;
           pure (oty.func (lift t1) t2, oexp.abst x (lift t1) e')
       | exp.app e1 e2 =>
-          '(tf, e1') <- synth e1 Γ ;;
+          '(tf, e1') <- osynth e1 Γ ;;
           τ1         <- pick ;;
           τ2         <- pick ;;
           _          <- equals tf[_] (oty.func τ1[_] τ2) ;;
-          e2'        <- check e2 Γ[_] τ1[_] ;;
+          e2'        <- ocheck e2 Γ[_] τ1[_] ;;
           pure (τ2[_], oexp.app e1'[_] e2')
       end.
 
@@ -119,11 +121,12 @@ Section Generator.
   Context {wpM : WeakestPre Θ M} {wlpM : WeakestLiberalPre Θ M}
     {tcLogicM : TypeCheckLogicM Θ M}.
 
-  Definition TPB_algo : ⊧ OEnv ⇢ Const Exp ⇢ OTy ⇢ OExp ⇢ Pred :=
+  Definition otyping_algo_synth : ⊧ OEnv ⇢ Const Exp ⇢ OTy ⇢ OExp ⇢ Pred :=
     fun w0 G0 e t0 e0 =>
-    WP (synth e G0)
+    WP (osynth e G0)
       (fun w1 (θ1 : Θ w0 w1) '(t1,e1) =>
          t0[θ1] =ₚ t1 /\ₚ e0[θ1] =ₚ e1).
+  Notation "Γ |--ₐ e ↓ t ~> e'" := (otyping_algo_synth Γ e t e') (at level 75).
 
   Goal False. Proof.
   Ltac wlpauto :=
@@ -132,12 +135,12 @@ Section Generator.
        try
          match goal with
          | H: _ /\ _ |- _ => destruct H
-         | IH: forall w G, bi_emp_valid (WLP (synth ?e G) _)
-           |- environments.envs_entails _ (WLP (synth ?e ?G) _) =>
+         | IH: forall w G, bi_emp_valid (WLP (osynth ?e G) _)
+           |- environments.envs_entails _ (WLP (osynth ?e ?G) _) =>
              iApply (wlp_mono' $! (IH _ G));
              iIntros (?w ?θ) "!>"; iIntros ([?t ?e']) "#?"
-         | IH: forall w G τ, bi_emp_valid (WLP (check ?e G τ) _)
-           |- environments.envs_entails _ (WLP (check ?e ?G ?τ) _) =>
+         | IH: forall w G τ, bi_emp_valid (WLP (ocheck ?e G τ) _)
+           |- environments.envs_entails _ (WLP (ocheck ?e ?G ?τ) _) =>
              iApply (wlp_mono' $! (IH _ G τ));
              iIntros (?w ?θ) "!>"; iIntros (?e') "#?"
          | |- environments.envs_entails _ (TPB _ _ _ _) =>
@@ -153,15 +156,15 @@ Section Generator.
          match goal with
          | H: _ /\ _ |- _ => destruct H
          | IH: forall (w : World) (G : OEnv w) (t : OTy w),
-             bi_emp_valid (bi_impl _ (bi_impl _ (WP (check ?e G t) _)))
-             |- environments.envs_entails _ (WP (check ?e ?G ?t) _) =>
+             bi_emp_valid (bi_impl _ (bi_impl _ (WP (ocheck ?e G t) _)))
+             |- environments.envs_entails _ (WP (ocheck ?e ?G ?t) _) =>
              iPoseProof (IH _ G t with "[] []") as "-#IH"; clear IH;
              [ | | iApply (wp_mono' with "IH");
                    iIntros (?w ?θ) "!>"; iIntros (?e') "#?"
              ]
          | IH: forall _ G,
-             bi_emp_valid (bi_impl _ (WP (synth ?e G) _))
-             |- environments.envs_entails _ (WP (synth ?e ?G) _) =>
+             bi_emp_valid (bi_impl _ (WP (osynth ?e G) _))
+             |- environments.envs_entails _ (WP (osynth ?e ?G) _) =>
              iPoseProof (IH _ G with "[]") as "-#IH"; clear IH;
              [| iApply (wp_mono' with "IH");
                 iIntros (?w ?θ) "!>";
@@ -170,11 +173,11 @@ Section Generator.
          end).
   Abort.
 
-  Lemma sound_aux e :
+  Lemma osoundness_aux e :
     (∀ w (G : OEnv w) (t : OTy w),
-        ⊢ WLP (check e G t) (fun _ θ ee => G[θ] |--ₚ e; t[θ] ~> ee)) /\
+        ⊢ WLP (ocheck e G t) (fun _ θ ee => G[θ] |--ₚ e; t[θ] ~> ee)) /\
     (∀ w (G : OEnv w),
-        ⊢ WLP (synth e G) (fun _ θ '(t,ee) => G[θ] |--ₚ e; t ~> ee)).
+        ⊢ WLP (osynth e G) (fun _ θ '(t,ee) => G[θ] |--ₚ e; t ~> ee)).
   Proof.
     induction e; cbn; (split; [intros w G τ|intros w G]); iStartProof; wlpauto.
     - destruct lookup eqn:HGx; wlpauto. iStopProof; pred_unfold.
@@ -183,23 +186,23 @@ Section Generator.
       constructor. now rewrite lookup_inst HGx.
   Qed.
 
-  Lemma sound (e : Exp) (w0 : World) (G0 : OEnv w0) t0 e0 :
-    TPB_algo G0 e t0 e0 ⊢ₚ G0 |--ₚ e; t0 ~> e0.
+  Lemma osoundness (e : Exp) (w0 : World) (G0 : OEnv w0) t0 e0 :
+    G0 |--ₐ e ↓ t0 ~> e0  ⊢ₚ  G0 |--ₚ e; t0 ~> e0.
   Proof.
     iStartProof. rewrite wand_is_impl. iApply wp_impl.
-    destruct (@sound_aux e) as [_ Hsound].
+    destruct (@osoundness_aux e) as [_ Hsound].
     iApply (wlp_mono' $! (@Hsound w0 G0)).
     iIntros "%w1 %θ1 !>" ([t e']) "HT". predsimpl.
     iStopProof; pred_unfold. intros HT Heq1 Heq2. now subst.
   Qed.
 
-  Lemma complete_aux {G e t ee} (T : G |-- e ∷ t ~> ee) :
+  Lemma ocompleteness_aux {G e t ee} (T : G |-- e ∷ t ~> ee) :
     (∀ w0 (G0 : OEnv w0) (t0 : OTy w0),
       ⊢ lift G =ₚ G0 ->ₚ lift t =ₚ t0 ->ₚ
-        WP (check e G0 t0) (fun _ _ e' => Open.pure ee =ₚ e')%P) /\
+        WP (ocheck e G0 t0) (fun _ _ e' => Open.pure ee =ₚ e')%P) /\
     (∀ w0 (G0 : OEnv w0),
       ⊢ lift G =ₚ G0 →
-        WP (synth e G0) (fun _ _ '(t',e') => lift t =ₚ t' /\ₚ Open.pure ee =ₚ e')%P).
+        WP (osynth e G0) (fun _ _ '(t',e') => lift t =ₚ t' /\ₚ Open.pure ee =ₚ e')%P).
   Proof.
     induction T; cbn; (split; [intros ? G0 ?|intros ? G0]); iStartProof; wpauto.
     - destruct (G0 !! _) eqn:HGx; wpauto.
@@ -213,18 +216,18 @@ Section Generator.
         intros ? ->; rewrite lookup_inst HGx in H; cbn in H; congruence.
   Qed.
 
-  Lemma complete (e : Exp) (w0 : World) (G0 : OEnv w0) t0 e0 :
-    G0 |--ₚ e; t0 ~> e0 ⊢ₚ TPB_algo G0 e t0 e0.
+  Lemma ocompleteness (e : Exp) (w0 : World) (G0 : OEnv w0) t0 e0 :
+    G0 |--ₚ e; t0 ~> e0  ⊢ₚ  G0 |--ₐ e ↓ t0 ~> e0.
   Proof.
-    pred_unfold. intros ι HT. destruct (complete_aux HT) as [_ Hcompl].
+    pred_unfold. intros ι HT. destruct (ocompleteness_aux HT) as [_ Hcompl].
     specialize (Hcompl _ G0). destruct Hcompl as [Hcompl].
     specialize (Hcompl ι (MkEmp _)). pred_unfold. rewrite inst_lift in Hcompl.
     specialize (Hcompl eq_refl). revert Hcompl. apply wp_mono.
     intros w1 θ1 ι1 <- [τ1 e1]. pred_unfold.
   Qed.
 
-  Lemma correct {w} (Γ : OEnv w) (e : Exp) (τ : OTy w) (e' : OExp w) :
-    Γ |--ₚ e; τ ~> e' ⊣⊢ₚ TPB_algo Γ e τ e'.
-  Proof. iSplit. iApply complete. iApply sound. Qed.
+  Lemma ocorrectness {w} (Γ : OEnv w) (e : Exp) (τ : OTy w) (e' : OExp w) :
+    Γ |--ₚ e; τ ~> e'  ⊣⊢ₚ  Γ |--ₐ e ↓ τ ~> e'.
+  Proof. iSplit. iApply ocompleteness. iApply osoundness. Qed.
 
 End Generator.
