theories/Gen/Synthesise.v
@@ -44,8 +44,8 @@ Section Generator.
     {reflTransΘ: ReflTrans Θ}.
   Context `{pureM:Pure M, bindM:Bind Θ M, failM:Fail M, tcM:TypeCheckM M}.
 
-  Definition generate : Exp -> ⊧ OEnv ⇢ M (OTy * OExp) :=
-    fix gen e {w} Γ :=
+  Definition osynth : Exp -> ⊧ OEnv ⇢ M (OTy * OExp) :=
+    fix osynth e {w} Γ :=
       match e with
       | exp.var x =>
           match lookup x Γ with
@@ -55,22 +55,22 @@ Section Generator.
       | exp.true  => pure (oty.bool, oexp.true)
       | exp.false => pure (oty.bool, oexp.false)
       | exp.ifte e1 e2 e3 =>
-          '(t1,e1') <- gen e1 Γ ;;
-          '(t2,e2') <- gen e2 Γ[_] ;;
-          '(t3,e3') <- gen e3 Γ[_] ;;
+          '(t1,e1') <- osynth e1 Γ ;;
+          '(t2,e2') <- osynth e2 Γ[_] ;;
+          '(t3,e3') <- osynth e3 Γ[_] ;;
           _         <- equals oty.bool t1[_] ;;
           _         <- equals t2[_] t3[_] ;;
           pure (t3[_], oexp.ifte e1'[_] e2'[_] e3'[_])
       | exp.absu x e =>
           t1       <- pick ;;
-          '(t2,e') <- gen e (insert (M := OEnv _) x t1 Γ[_]) ;;
+          '(t2,e') <- osynth e (insert (M := OEnv _) x t1 Γ[_]) ;;
           pure (oty.func t1[_] t2, oexp.abst x t1[_] e')
       | exp.abst x t1 e =>
-          '(t2,e') <- gen e (insert (M := OEnv _) x (lift t1) Γ) ;;
+          '(t2,e') <- osynth e (insert (M := OEnv _) x (lift t1) Γ) ;;
           pure (oty.func (lift t1) t2, oexp.abst x (lift t1) e')
       | exp.app e1 e2 =>
-          '(tf, e1') <- gen e1 Γ ;;
-          '(t1, e2') <- gen e2 Γ[_] ;;
+          '(tf, e1') <- osynth e1 Γ ;;
+          '(t1, e2') <- osynth e2 Γ[_] ;;
           t2 <- pick ;;
           _  <- equals tf[_] (oty.func t1[_] t2) ;;
           pure (t2[_], oexp.app e1'[_] e2'[_])
@@ -82,17 +82,18 @@ Section Generator.
   Context {wpM : WeakestPre Θ M} {wlpM : WeakestLiberalPre Θ M}
     {tcLogicM : TypeCheckLogicM Θ M}.
 
-  Definition TPB_algo : ⊧ OEnv ⇢ Const Exp ⇢ OTy ⇢ OExp ⇢ Pred :=
+  Definition otyping_algo : ⊧ OEnv ⇢ Const Exp ⇢ OTy ⇢ OExp ⇢ Pred :=
     fun w0 G0 e t0 e0 =>
-    WP (generate e G0)
+    WP (osynth e G0)
       (fun w1 (θ1 : Θ w0 w1) '(t1,e1) =>
          t0[θ1] =ₚ t1 /\ₚ e0[θ1] =ₚ e1).
+  Notation "Γ |--ₐ e ∷ t ~> e'" := (otyping_algo Γ e t e') (at level 80).
 
   Goal False. Proof.
   Ltac wlpindhyp :=
     match goal with
-    | IH: ∀ w G, bi_emp_valid (WLP (generate ?e G) _)
-      |- environments.envs_entails _ (WLP (generate ?e ?G) _) =>
+    | IH: ∀ w G, bi_emp_valid (WLP (osynth ?e G) _)
+      |- environments.envs_entails _ (WLP (osynth ?e ?G) _) =>
         iApply (wlp_mono' $! (IH _ G));
         iIntros (?w ?θ) "!>"; iIntros ([?t ?e']) "#?"; clear IH
     | |- environments.envs_entails _ (TPB _ _ _ _) =>
@@ -103,8 +104,8 @@ Section Generator.
   Ltac wpindhyp :=
     match goal with
     | IH: forall _ G,
-        bi_emp_valid (bi_impl _ (WP (generate ?e G) _))
-      |- environments.envs_entails _ (WP (generate ?e ?G) _) =>
+        bi_emp_valid (bi_impl _ (WP (osynth ?e G) _))
+      |- environments.envs_entails _ (WP (osynth ?e ?G) _) =>
         iPoseProof (IH _ G with "[]") as "-#IH"; clear IH;
         [| iApply (wp_mono' with "IH");
            iIntros (?w ?θ) "!>";
@@ -114,11 +115,10 @@ Section Generator.
   Ltac wpauto := repeat (repeat wpsimpl; try wpindhyp).
   Abort.
 
-  Lemma generate_sound_aux e :
+  Lemma osoundness_aux e :
     ∀ w (G : OEnv w),
-      ⊢ WLP (generate e G) (fun _ θ '(t,ee) => G[θ] |--ₚ e; t ~> ee).
-    (*
-  Proof with
+      ⊢ WLP (osynth e G) (fun _ θ '(t,ee) => G[θ] |--ₚ e; t ~> ee).
+  (* Proof with
     iStopProof; pred_unfold; intuition (subst; econstructor; eauto; fail).
     induction e; cbn; intros w G; iStartProof.
     - destruct lookup eqn:HGx; wlpauto.
@@ -135,27 +135,26 @@ Section Generator.
       iApply wlp_equals.
       (* Assume that the equality holds on the ghost state (assignment). *)
       iIntros "#?".
-      (* The rule for equality is generalized with the ◼ modality to
-         allow different behaviour from the monad. The Free monad implementation
-         of equals always calls the continuation with the identity substitution.
-         However, the solved monad calls the unifier and hence the continuation
-         is called with some substitution that we cannot know upfront. Of course,
-         we do not want to make the unifier part of the semantics of the wlp rule
-         for equals either. Hence the use of the ◼ modality that requires us to
-         show the postcondition for any substitution. *)
+      (* The rule for equality is generalized with the ◼ modality to *)
+      (* allow different behaviour from the monad. The Free monad implementation *)
+      (* of equals always calls the continuation with the identity substitution. *)
+      (* However, the solved monad calls the unifier and hence the continuation *)
+      (* is called with some substitution that we cannot know upfront. Of course, *)
+      (* we do not want to make the unifier part of the semantics of the wlp rule *)
+      (* for equals either. Hence the use of the ◼ modality that requires us to *)
+      (* show the postcondition for any substitution. *)
       unfold PBox.  (* PBox is defined using Sub.wlp. *)
       iIntros (?w ?θ).
-      (* Introduce the wlp from the head by running the substitution
-         over the context. *)
+      (* Introduce the wlp from the head by running the substitution *)
+      (* over the context. *)
       iModIntro.
-      (* The modality introduction uses typeclass-based logic programming to
-         perform some rewrites. For instance, the barebones modality introduction
-         of the wlp would result in the last assumption to be the constraint
-           (oty.bool =ₚ t[θ0 ⊙ θ1])[θ2]
-         but the typeclass machinery automatically "rewrote" it to
-           oty.bool[θ2] =ₚ t[θ0 ⊙ θ1][θ2]
-         Similarly, for the typing judgements.
-       *)
+      (* The modality introduction uses typeclass-based logic programming to *)
+      (* perform some rewrites. For instance, the barebones modality introduction *)
+      (* of the wlp would result in the last assumption to be the constraint *)
+      (*   (oty.bool =ₚ t[θ0 ⊙ θ1])[θ2] *)
+      (* but the typeclass machinery automatically "rewrote" it to *)
+      (*   oty.bool[θ2] =ₚ t[θ0 ⊙ θ1][θ2] *)
+      (* Similarly, for the typing judgements. *)
       iApply wlp_bind.
       iApply wlp_equals. iIntros "#?". iIntros (?w ?θ) "!>".
       iApply wlp_pure...
@@ -176,39 +175,39 @@ Section Generator.
       iApply wlp_bind.
       iApply wlp_equals. iIntros "#?". iIntros (?w ?θ) "!>".
       iApply wlp_pure.
-      (* Unfortunately, we are accumulating a lot of substitutions in the goal.
-         We can make the output nicer through generalizations. *)
+      (* Unfortunately, we are accumulating a lot of substitutions in the goal. *)
+      (* We can make the output nicer through generalizations. *)
       rewrite ?subst_trans; predsimpl.
-      (* The subst_trans doesn't work for the elaboration because that would
-         need either functional extensionality or a generalized rewrite *)
-      (* At this point we would like to apply the typing relation for the
-         application case. However, we did not define it for the open typing
-         relation. So at this point we the "base logic" abstraction and go to
-         the underlying definition of predicates and also to the closed typing
-         relation that underlies the open typing relation. We can generalize
-         the result further to get rid of more substitutions. *)
+      (* The subst_trans doesn't work for the elaboration because that would *)
+      (* need either functional extensionality or a generalized rewrite *)
+      (* At this point we would like to apply the typing relation for the *)
+      (* application case. However, we did not define it for the open typing *)
+      (* relation. So at this point we the "base logic" abstraction and go to *)
+      (* the underlying definition of predicates and also to the closed typing *)
+      (* relation that underlies the open typing relation. We can generalize *)
+      (* the result further to get rid of more substitutions. *)
       iStopProof. pred_unfold.
       (* Use the typing rule of the closed typing relation. *)
       intuition (subst; econstructor; eauto; fail).
-  *)
+  Restart. *)
   Proof.
     induction e; cbn; intros w G; iStartProof; wlpauto.
     destruct lookup eqn:HGx; wlpauto. iStopProof; pred_unfold.
     constructor. now rewrite lookup_inst HGx.
   Qed.
 
-  Lemma generate_sound (e : Exp) {w0} (G0 : OEnv w0) t0 e0 :
-    TPB_algo G0 e t0 e0 ⊢ₚ G0 |--ₚ e; t0 ~> e0.
+  Lemma osoundness (e : Exp) {w} (Γ : OEnv w) τ e' :
+    Γ |--ₐ e ∷ τ ~> e'  ⊢ₚ  Γ |--ₚ e; τ ~> e'.
   Proof.
     iStartProof. rewrite wand_is_impl. iApply wp_impl.
-    iApply (wlp_mono' $! (@generate_sound_aux e w0 G0)).
-    iIntros "%w1 %θ1 !>" ([t e']) "HT". iStopProof; pred_unfold.
+    iApply (wlp_mono' $! (@osoundness_aux e w Γ)).
+    iIntros "%w1 %θ1 !>" ([τ' e'']) "HT". iStopProof; pred_unfold.
     intros HT [Heq1 Heq2]. now subst.
   Qed.
 
-  Lemma generate_complete_aux {G e t ee} (T : G |-- e ∷ t ~> ee) :
+  Lemma ocompleteness_aux {G e t ee} (T : G |-- e ∷ t ~> ee) :
     ∀ w0 (G0 : OEnv w0), ⊢ lift G =ₚ G0 →
-      WP (generate e G0)
+      WP (osynth e G0)
           (fun _ _ '(t',e') => lift t =ₚ t' /\ₚ Open.pure ee =ₚ e')%P.
   Proof.
     induction T; cbn; intros w0 G0; iStartProof; wpauto.
@@ -216,11 +215,11 @@ Section Generator.
       intros ? ->; rewrite lookup_inst HGx in H; cbn in H; congruence.
   Qed.
 
-  Lemma generate_complete {w} (Γ : OEnv w) (e : Exp) (τ : OTy w) (e' : OExp w) :
-    Γ |--ₚ e; τ ~> e' ⊢ₚ TPB_algo Γ e τ e'.
+  Lemma ocompleteness {w} (Γ : OEnv w) (e : Exp) (τ : OTy w) (e' : OExp w) :
+    Γ |--ₚ e; τ ~> e'  ⊢ₚ  Γ |--ₐ e ∷ τ ~> e'.
   Proof.
     pred_unfold. intros ι HT.
-    destruct (generate_complete_aux HT Γ) as [Hcompl].
+    destruct (ocompleteness_aux HT Γ) as [Hcompl].
     specialize (Hcompl ι (MkEmp _)). pred_unfold.
     rewrite inst_lift in Hcompl.
     specialize (Hcompl eq_refl). revert Hcompl.
@@ -228,8 +227,8 @@ Section Generator.
     pred_unfold.
   Qed.
 
-  Lemma generate_correct {w} (Γ : OEnv w) (e : Exp) (τ : OTy w) (e' : OExp w) :
-    Γ |--ₚ e; τ ~> e' ⊣⊢ₚ TPB_algo Γ e τ e'.
-  Proof. iSplit. iApply generate_complete. iApply generate_sound. Qed.
+  Lemma ocorrectness {w} (Γ : OEnv w) (e : Exp) (τ : OTy w) (e' : OExp w) :
+    Γ |--ₚ e; τ ~> e'  ⊣⊢ₚ  Γ |--ₐ e ∷ τ ~> e'.
+  Proof. iSplit. iApply ocompleteness. iApply osoundness. Qed.
 
 End Generator.
